## The variance, covariance, correlation and linear equation


### The empirical **variance**

$$
\begin{eqnarray*}
Var(X)
 & = & \frac{1}{n - 1}\sum_{i = 1}^n(X_i - \bar X)^2\\
 & = & \frac{1}{n - 1}\sum_{i = 1}^n(X_i^2 - 2X_i\bar X + \bar X^2)\\
 & = & \frac{1}{n - 1}\left(\sum_{i = 1}^nX_i^2 - 2\bar X\sum_{i = 1}^nX_i + \sum_{i = 1}^n\bar X^2\right)\\
 & = & \frac{1}{n - 1}\left(\sum_{i = 1}^nX_i^2 - 2\bar Xn\bar X + n\bar X^2\right)\\
 & = & \frac{1}{n - 1}\left(\sum_{i = 1}^nX_i^2 - 2n\bar X^2 + n\bar X^2\right)\\
 & = & \frac{1}{n - 1}\left(\sum_{i = 1}^nX_i^2 - n\bar X^2\right)
\end{eqnarray*}
$$

### The empirical **standard deviation**

$$
Sd(X) = \sqrt {Var(X)}
$$

### The empirical **covariance**

$$
\begin{eqnarray*}
Cov(X, Y) 
 & = & \frac{1}{n - 1}\sum_{i = 1}^n(X_i - \bar X)(Y_i - \bar Y)\\
 & = & \frac{1}{n - 1}\sum_{i = 1}^n(X_iY_i - X_i\bar Y  - \bar XY_i + \bar X\bar Y)\\
 & = & \frac{1}{n - 1}\left(\sum_{i = 1}^nX_iY_i - \bar Y\sum_{i = 1}^nX_i - \bar X\sum_{i = 1}^nY_i + \sum_{i = 1}^n\bar X\bar Y\right)\\
 & = & \frac{1}{n - 1}\left(\sum_{i = 1}^nX_iY_i - \bar Yn\bar X - \bar Xn\bar Y + n\bar X\bar Y\right)\\
 & = & \frac{1}{n - 1}\left(\sum_{i = 1}^nX_iY_i - n\bar X\bar Y - n\bar X\bar Y + n\bar X\bar Y\right)\\
 & = & \frac{1}{n - 1}\left(\sum_{i = 1}^nX_iY_i - n\bar X\bar Y\right)
\end{eqnarray*}
$$

### The **correlation**

$$
Cor(X, Y) = \frac{Cov(X, Y)}{Sd(X)Sd(Y)}
$$

### The linear equation

$$
Y = \beta_0 + \beta_1X
$$

$$
\hat\beta_1 = Cor(Y, X)\frac{Sd(Y)}{Sd(X)}
$$

$$
\hat\beta_0 = \bar Y - \beta_1\bar X
$$

To go further:

$$
\begin{eqnarray*}
\hat\beta_1 
 & = & Cor(Y, X)\frac{Sd(Y)}{Sd(X)}\\
 & = & \frac{Cov(Y, X)}{Sd(X)Sd(Y)}\frac{Sd(Y)}{Sd(X)}\\
 & = & \frac{Cov(Y, X)}{Sd(X)^2}\\
 & = & \frac{Cov(Y, X)}{Var(X)}\\
 & = & \frac{\frac{1}{n - 1}\left(\sum_{i = 1}^nX_iY_i - n\bar X\bar Y\right)}{\frac{1}{n - 1}\left(\sum_{ i = 1}^nX_i^2 - n\bar X^2\right)}\\
 & = & \frac{\sum_{i = 1}^nX_iY_i - n\bar X\bar Y}{\sum_{ i = 1}^nX_i^2 - n\bar X^2}
 \end{eqnarray*}
$$

Even further:

$$
\begin{eqnarray*}
\hat\beta_1 
 & = & \frac{\sum_{i = 1}^nX_iY_i - n\bar X\bar Y}{\sum_{ i = 1}^nX_i^2 - n\bar X^2}\\
  & = & \frac{\sum_{i = 1}^nX_iY_i - n\frac{\sum_{i = 1}^nX_i}{n}\frac{\sum_{i = 1}^nY_i}{n}}{\sum_{ i = 1}^nX_i^2 - n\left(\frac{\sum_{i = 1}^nX_i}{n}\right)^2}\\
  & = & \frac{n\sum_{i = 1}^nX_iY_i - \sum_{i = 1}^nX_i\sum_{i = 1}^nY_i}{n\sum_{ i = 1}^nX_i^2 - \left(\sum_{i = 1}^nX_i\right)^2}
\end{eqnarray*}
$$

That is the equation given by edX course *I Heart Stats*.

> Note: for **centered** data, both $\bar X$ and $\bar Y$ are 0; for **scaled** and **normalized** data, both $Sd(X)$ and $Sd(Y)$ are 1.
 
